theories/semantics.v
@@ -4,9 +4,11 @@ Require Import syntax core fintype.
 From HB Require Import structures.
 
 (* notations for proc here*)
-
+(*
 Open Scope subst_scope.
-
+*)
+  #[global]
+  Open Scope subst_scope.
 Definition var_one {n : nat} : fin (S (S n)) := shift var_zero.
 Definition var_two {n : nat} : fin (S (S (S n))) := shift var_one.
 Definition var_three {n : nat} : fin (S (S (S (S n)))) := shift var_two.
@@ -30,6 +32,9 @@ Notation "x ? ․ P" := (WaitP x P) (at level 44, right associativity).
 Notation "x ! ․ P" := (CloseP x P) (at level 44, right associativity).
 Notation "x ! y ․ P" := (DelP x y P) (at level 44, right associativity).
 
+Notation "< sigma_ch >" := (subst_proc sigma_ch).
+Notation "s .: sigma" := (scons s sigma) (at level 55, sigma at next level, right associativity) : subst_scope.
+Notation "s '..'" := (scons s ids) (at level 1, format "s ..") : subst_scope.
 
 (* Decidability of equality on fin and ch *) 
 Arguments var_ch {n_ch}.
@@ -72,19 +77,97 @@ HB.instance Definition _ n := hasDecEq.Build (ch n) ch_eqP.
 
 
 (* substitutions on processes *) 
+(* am: unused
 Definition shift_up {m:nat} := 
   subst_proc (fun (x:fin m) => (var_ch (shift x))).
-
+*)
 Definition shift_two_up {m:nat} := 
   subst_proc (fun (x:fin m) => (var_ch (shift(shift x)))).
 
-Definition swap_ch {m_ch : nat} (n1 n2 : fin m_ch) :=
+Definition swap_ch {m : nat} (n1 n2 : fin m) :=
   fun n => var_ch (if n == n1 then n2 else if n == n2 then n1 else n). 
 
 
 
-(* Structural Equivalence (or Congruence) *) 
+
+(* Structural Equivalence (or Congruence) *)
+Reserved Notation "P '≅' Q" (at level 60, right associativity).
+(* StartSE *)
 Inductive struct_eq {n:nat} : proc n -> proc n -> Prop :=
+    SC_Par_Com : forall P Q : proc n,
+                 P ∥ Q ≅ Q ∥ P            
+  | SC_Par_Assoc : forall P Q R : proc n,
+                   P ∥ Q ∥ R ≅ P ∥ (Q ∥ R)
+  | SC_Par_Inact : forall P : proc n,
+                   P ∥ ∅ ≅ P
+  | SC_Res_Scope : forall (P : proc n.+2) (Q : proc n),
+                   (ν) P ∥ Q ≅  (ν) (P ∥ shift_two_up Q)
+  | SC_Res_SwapC : forall P : proc n.+2,
+                   (ν) P ≅ (ν) (< swap_ch var_zero var_one >) P                  
+  | SC_Res_SwapB : forall P : proc n.+4,
+                   (ν) (ν) P ≅ (ν) (ν) (< swap_ch var_one var_three >)
+                     ((< swap_ch var_zero var_two >) P) 
+                     (* EndSE *)
+(* StartInact *)
+  | SC_Res_Inact : (ν) ∅ ≅ ∅  
+  (* EndInact *)                                  
+  | SC_Refl : forall P : proc n, P ≅ P
+  | SC_Sym : forall P Q : proc n,
+             P ≅ Q -> Q ≅ P
+  | SC_Trans : forall P Q R : proc n,
+               P ≅ Q -> Q ≅ R -> P ≅ R
+  | SC_Cong_Par : forall
+                    P P' Q Q' : proc n,
+                  P ≅ P' ->
+                  Q ≅ Q' ->
+                  P ∥ Q ≅ P' ∥ Q'
+  | SC_Cong_Res : forall
+                    P P' : proc n.+2,
+                  P ≅ P' ->
+                  (ν) P ≅ (ν) P'
+  | SC_Cong_Close : forall
+                      (P P' : proc n)
+                      (x : ch n),
+                    P ≅ P' ->
+                    x ! ․ P ≅ x ! ․ P'
+  | SC_Cong_Wait : forall
+                     (P P' : proc n)
+                     (x : ch n),
+                   P ≅ P' ->
+                   x ? ․ P ≅ x ? ․ P'
+  | SC_Cong_OutS : forall
+                     (P P' : proc n)
+                     (x y : ch n),
+                   P ≅ P' ->
+                   x ! y ․ P
+                   ≅ x ! y ․ P'
+  | SC_Cong_InsP : forall
+                     (P P' : proc n.+1)
+                     (x : ch n),
+                   P ≅ P' ->
+                   x ? (_)․P
+                   ≅ x ? (_)․P'
+                   where   "P '≅' Q" := (struct_eq P Q).
+                   
+
+(*
+  fun i => match i with
+  | None => var_ch var_zero           (* 0 maps to 0 in scope n *)
+  | Some None => var_ch var_zero      (* 1 also maps to 0 (they're connected) *)
+  | Some (Some j) => var_ch (Some j)  (* channels 2+ shift down by 1 *)
+  end.                   
+Definition close_subst {n : nat} : fin n.+2 -> ch n :=
+  fun i => match i with
+  | None => var_ch None           (* 0 maps to 0 in the lower scope *)
+  | Some None => var_ch None      (* 1 also maps to 0 (they're connected) *)
+  | Some (Some j) => var_ch (j)  (* other channels shift down by 2 *)
+  end.
+Definition close_subst {n : nat} : fin n.+2 -> ch n :=
+  fun i => match i with
+  | None => var_ch n None           (* 0 maps to 0 in the lower scope *)
+  | Some None => var_ch n None      (* 1 also maps to 0 (they're connected) *)
+  | Some (Some j) => var_ch n (Some j)  (* other channels shift down by 2 *)
+  end.
 
 | SC_Par_Com P Q     : struct_eq (ParP P Q) (ParP Q P) 
 
@@ -102,8 +185,7 @@ Inductive struct_eq {n:nat} : proc n -> proc n -> Prop :=
 | SC_Res_SwapB P : struct_eq (ResP (ResP P))
                      (ResP (ResP (subst_proc (swap_ch var_one var_three)
                                     (subst_proc (swap_ch var_zero var_two) 
-                                       P)) 
-                     )) 
+                                       P)))) 
 
 (* equivalence rules *) 
 | SC_Refl P          : struct_eq P P
@@ -118,11 +200,25 @@ Inductive struct_eq {n:nat} : proc n -> proc n -> Prop :=
 | SC_Cong_OutS P P' x  y : struct_eq P P' -> struct_eq (DelP x y P) (DelP x y P')
 | SC_Cong_InsP P P' x    : struct_eq P P' -> struct_eq (InSP x  P) (InSP x  P')
 .
+*)
 
-Notation   "P '≅' Q" := (struct_eq P Q) (at level 60, right associativity).
 
-
+Reserved Notation " P '⇛' Q " (at level 50, left associativity).  
+      (* StartRed *)
 Inductive reduce {n:nat} : proc n -> proc n -> Prop :=
+  | R_Res : forall P Q : proc n.+2,
+            P ⇛ Q -> (ν) P ⇛ (ν) Q
+  | R_Par : forall P Q R : proc n,
+            P ⇛ Q -> P ∥ R ⇛ Q ∥ R
+  | R_Struct : forall P P' Q Q' : proc n,
+               P ≅ P' -> P' ⇛ Q' -> Q' ≅ Q -> P ⇛ Q
+  | R_Close : forall P Q : proc n.+2,
+             (ν) (1 ! ․ P ∥ 0 ? ․ Q) ⇛ ((ν) (P ∥ Q)) 
+  | R_Com : forall (x : ch n.+2)(P : proc n.+2) (Q : proc n.+3),
+            (ν) (1 ! x ․ P ∥ 0 ? (_)․Q) ⇛ (ν) (P ∥ (< x.. >) Q) (* EndRed *)
+            
+where " P '⇛' Q " := (reduce P Q) . Check ids.
+(*
 | R_Res P Q          : reduce P Q ->
                        reduce (ResP P) (ResP Q)
 
@@ -142,8 +238,5 @@ Inductive reduce {n:nat} : proc n -> proc n -> Prop :=
 | R_Del x P Q:        
   reduce (ResP (ParP (DelP (var_ch var_one) x P) 
                   (InSP (var_ch var_zero)   Q) ))
-    (ResP (ParP P (subst_proc (scons x ids) Q) ))
-.
-
-
-Notation " P '⇛' Q " := (reduce P Q) (at level 50, left associativity).  
+    (ResP (ParP P (subst_proc (scons x ids) Q) )) *)
+    
